src/SDK/Keyring/Defs.dfy
@@ -11,7 +11,9 @@ module {:extern "KeyringDefs"} KeyringDefs {
 
   trait {:termination false} Keyring {
     ghost var Repr : set<object>
-    predicate Valid() reads this, Repr
+    predicate Valid()
+      reads this, Repr
+      ensures Valid() ==> this in Repr
 
     method OnEncrypt(materials: Materials.ValidEncryptionMaterials) returns (res: Result<Materials.ValidEncryptionMaterials>)
       requires Valid()
